src/Resolute_JSON.v
@@ -6,6 +6,7 @@ Import ListNotations ResultNotation.
 
 Definition STR_RESOLUTE_SUCCESS : string := "RESOLUTE_POLICY_CHECK".
 Definition STR_RESOLUTE_FORMULA : string := "RESOLUTE_FORMULA".
+Definition STR_RESOLUTE_EVIDENCE : string := "RESOLUTE_EVIDENCE".
 
 Definition STR_RESOLUTE : string := "RESOLUTE".
 Definition r_false_name_constant : string := "R_False".
@@ -15,74 +16,38 @@ Definition r_and_name_constant : string := "R_And".
 Definition r_or_name_constant : string := "R_Or".
 Definition r_imp_name_constant : string := "R_Imp".
 
-Fixpoint Resolute_to_JSON (t : Resolute)  : JSON := 
+Definition r_goal_e_name_constant : string := "R_Goal_E".
+Definition r_and_e_name_constant : string := "R_And_E".
+Definition r_or_e_name_constant : string := "R_Or_E".
+
+Fixpoint Resolute_to_JSON (t : Resolute_Formula)  : JSON := 
   match t with
-  | R_False => constructor_to_JSON STR_RESOLUTE r_false_name_constant []
-  | R_True => constructor_to_JSON STR_RESOLUTE r_true_name_constant []
-  | R_Goal tid => constructor_to_JSON STR_RESOLUTE r_goal_name_constant [JSON_String (to_string tid)]
-  | R_And t1 t2 => constructor_to_JSON STR_RESOLUTE r_and_name_constant
+  | R_Goal tid args => constructor_to_JSON STR_RESOLUTE_FORMULA r_goal_name_constant [JSON_String (to_string tid); (to_JSON args)]
+  | R_And t1 t2 => constructor_to_JSON STR_RESOLUTE_FORMULA r_and_name_constant
   [(Resolute_to_JSON t1); (Resolute_to_JSON t2)]
-  | R_Or t1 t2 => constructor_to_JSON STR_RESOLUTE r_or_name_constant
+  | R_Or t1 t2 => constructor_to_JSON STR_RESOLUTE_FORMULA r_or_name_constant
   [(Resolute_to_JSON t1); (Resolute_to_JSON t2)]
-  | R_Imp t1 t2 => constructor_to_JSON STR_RESOLUTE r_imp_name_constant
-  [(Resolute_to_JSON t1); (Resolute_to_JSON t2)]
-  (*
-  | att p t' => constructor_to_JSON STR_TERM att_name_constant 
-      [(JSON_String (to_string p)); (Resolute_to_JSON t')]
-  | lseq t1 t2 => constructor_to_JSON STR_TERM lseq_name_constant
-      [(Resolute_to_JSON t1); (Resolute_to_JSON t2)]
-  | bseq sp t1 t2 => constructor_to_JSON STR_TERM bseq_name_constant
-      [(to_JSON sp); (Resolute_to_JSON t1); (Resolute_to_JSON t2)]
-  | bpar sp t1 t2 => constructor_to_JSON STR_TERM bpar_name_constant
-      [(to_JSON sp); (Resolute_to_JSON t1); (Resolute_to_JSON t2)]
-      *)
   end.
 
 Open Scope string_scope.
 
-Fixpoint Resolute_from_JSON (js : JSON) : ResultT Resolute string :=
-    let type_name := STR_RESOLUTE in
+Fixpoint Resolute_from_JSON (js : JSON) : ResultT Resolute_Formula string :=
+    let type_name := STR_RESOLUTE_FORMULA in
     let type_str := type_name ++ type_sep ++ type_string_constant in
     let body_str := type_name ++ type_sep ++ body_string_constant in
     match (JSON_get_Object type_str js) with
     | resultC (JSON_String cons_name) =>
-      if (eqb cons_name r_false_name_constant) 
-      then 
-        resultC R_False 
-      (*
-        asp_js <- (JSON_get_Object body_str js) ;;
-        asp_val <- from_JSON asp_js ;;
-        resultC (asp asp_val)
-      *)
-      else if (eqb cons_name r_true_name_constant) 
-      then 
-        resultC R_True
 
-      else if (eqb cons_name r_goal_name_constant) 
+      if (eqb cons_name r_goal_name_constant) 
       then 
       match (JSON_get_Object body_str js) with 
-      | resultC (JSON_String n_js) =>
+      | resultC (JSON_Array
+                  [(JSON_String n_js); args_js]) =>
           n <- from_string n_js ;;
-          resultC (R_Goal n)
+          args <- from_JSON args_js ;;
+          resultC (R_Goal n args)
         | _ => errC err_str_json_parsing_failure_wrong_number_args
         end
-      (*
-        body_js <- (JSON_get_Object body_str js) ;;
-        match body_js with
-        | JSON_Array [JSON_String n_js] => 
-          n <- from_string n_js ;;
-          resultC (R_Goal n)
-        | _ => errC err_str_json_parsing_failure_wrong_number_args
-        end
-        *)
-
-
-
-        (*
-        tid_val <- JSON_get_string 
-        tid_val <- from_string body_js ;;
-        resultC (R_Goal tid_val)
-        *)
 
       else if (eqb cons_name r_and_name_constant) 
       then match js with
@@ -107,58 +72,64 @@ Fixpoint Resolute_from_JSON (js : JSON) : ResultT Resolute string :=
             resultC (R_Or term1_val term2_val)
         | _ => errC err_str_json_parsing_failure_wrong_number_args
         end
+
+      else errC err_str_json_invalid_constructor_name
+    | resultC _ => errC err_str_json_invalid_constructor_name
+    | errC e => errC e
+    end.
+
+Fixpoint Resolute_Evidence_to_JSON `{Jsonifiable Evidence} (t : Resolute_Evidence)  : JSON := 
+  match t with
+  | R_Goal_E tid args e => constructor_to_JSON STR_RESOLUTE_EVIDENCE r_goal_e_name_constant [JSON_String (to_string tid); (to_JSON args); (to_JSON e)]
+  | R_And_E t1 t2 => constructor_to_JSON STR_RESOLUTE_EVIDENCE r_and_e_name_constant
+  [(Resolute_Evidence_to_JSON t1); (Resolute_Evidence_to_JSON t2)]
+  | R_Or_E t1 t2 => constructor_to_JSON STR_RESOLUTE_EVIDENCE r_or_e_name_constant
+  [(Resolute_Evidence_to_JSON t1); (Resolute_Evidence_to_JSON t2)]
+  end.
     
-      else if (eqb cons_name r_imp_name_constant) 
+Fixpoint Resolute_Evidence_from_JSON `{Jsonifiable Evidence} (js : JSON) : ResultT Resolute_Evidence string :=
+    let type_name := STR_RESOLUTE_EVIDENCE in
+    let type_str := type_name ++ type_sep ++ type_string_constant in
+    let body_str := type_name ++ type_sep ++ body_string_constant in
+    match (JSON_get_Object type_str js) with
+    | resultC (JSON_String cons_name) =>
+
+      if (eqb cons_name r_goal_e_name_constant) 
+      then 
+      match (JSON_get_Object body_str js) with 
+      | resultC (JSON_Array
+                  [(JSON_String n_js); args_js; e_js]) =>
+          n <- from_string n_js ;;
+          args <- from_JSON args_js ;;
+          e <- from_JSON e_js ;;
+          resultC (R_Goal_E n args e)
+        | _ => errC err_str_json_parsing_failure_wrong_number_args
+        end
+
+      else if (eqb cons_name r_and_e_name_constant) 
       then match js with
         | JSON_Object [
             _;
             (_, JSON_Array [ term1; term2 ])
           ] =>
-            term1_val <- (Resolute_from_JSON term1) ;;
-            term2_val <- (Resolute_from_JSON term2) ;;
-            resultC (R_Imp term1_val term2_val)
+            term1_val <- (Resolute_Evidence_from_JSON term1) ;;
+            term2_val <- (Resolute_Evidence_from_JSON term2) ;;
+            resultC (R_And_E term1_val term2_val)
         | _ => errC err_str_json_parsing_failure_wrong_number_args
         end
 
-
-
-        (*
-      else if (eqb cons_name lseq_name_constant) 
+      else if (eqb cons_name r_or_e_name_constant) 
       then match js with
         | JSON_Object [
             _;
             (_, JSON_Array [ term1; term2 ])
-         ] =>
-            term1_val <- (Term_from_JSON term1) ;;
-            term2_val <- (Term_from_JSON term2) ;;
-            resultC (lseq term1_val term2_val)
-        | _ => errC err_str_json_parsing_failure_wrong_number_args
-        end
-      else if (eqb cons_name bseq_name_constant) 
-      then match js with
-        | JSON_Object [
-            _;
-            (_, JSON_Array [ sp; term1; term2 ])
           ] =>
-            sp_val <- from_JSON sp ;;
-            term1_val <- (Term_from_JSON term1) ;;
-            term2_val <- (Term_from_JSON term2) ;;
-            resultC (bseq sp_val term1_val term2_val)
+            term1_val <- (Resolute_Evidence_from_JSON term1) ;;
+            term2_val <- (Resolute_Evidence_from_JSON term2) ;;
+            resultC (R_Or_E term1_val term2_val)
         | _ => errC err_str_json_parsing_failure_wrong_number_args
         end
-      else if (eqb cons_name bpar_name_constant) 
-      then match js with
-        | JSON_Object [
-            _;
-            (_, JSON_Array [ sp; term1; term2 ])
-         ] =>
-            sp_val <- from_JSON sp ;;
-            term1_val <- (Term_from_JSON term1) ;;
-            term2_val <- (Term_from_JSON term2) ;;
-            resultC (bpar sp_val term1_val term2_val)
-        | _ => errC err_str_json_parsing_failure_wrong_number_args
-        end
-        *)
+
       else errC err_str_json_invalid_constructor_name
     | resultC _ => errC err_str_json_invalid_constructor_name
     | errC e => errC e
@@ -166,21 +137,28 @@ Fixpoint Resolute_from_JSON (js : JSON) : ResultT Resolute string :=
 
 Close Scope string_scope.
 
-Global Instance Jsonifiable_Resolute : Jsonifiable Resolute. 
+Global Instance Jsonifiable_Resolute : Jsonifiable Resolute_Formula. 
 eapply Build_Jsonifiable with (to_JSON := Resolute_to_JSON) (from_JSON := Resolute_from_JSON).
 induction a; 
 repeat (result_monad_unfold;
 jsonifiable_hammer; repeat rewrite canonical_jsonification in *; eauto).
 Defined.
 
-Definition ResoluteResponse_to_JSON `{Jsonifiable Term, Jsonifiable Resolute} (resp:ResoluteResponse) : JSON := 
+Global Instance Jsonifiable_Resolute_Evidence : Jsonifiable Resolute_Evidence. 
+eapply Build_Jsonifiable with (to_JSON := Resolute_Evidence_to_JSON) (from_JSON := Resolute_Evidence_from_JSON).
+induction a; 
+repeat (result_monad_unfold;
+jsonifiable_hammer; repeat rewrite canonical_jsonification in *; eauto).
+Defined.
+
+Definition ResoluteResponse_to_JSON `{Jsonifiable Term, Jsonifiable Resolute_Formula} (resp:ResoluteResponse) : JSON := 
 
   JSON_Object 
     [(STR_RESOLUTE_SUCCESS, (JSON_Boolean (resoluteresp_success resp)));
     (STR_RESOLUTE_FORMULA, (to_JSON (resoluteresp_formula resp)));
     (STR_TERM, (to_JSON (resoluteresp_term resp)))].
 
-Definition ResoluteResponse_from_JSON `{Jsonifiable Term, Jsonifiable Resolute}
+Definition ResoluteResponse_from_JSON `{Jsonifiable Term, Jsonifiable Resolute_Formula}
 (resp:JSON) : ResultT ResoluteResponse string := 
   temp_success <- JSON_get_bool STR_RESOLUTE_SUCCESS resp ;;
   temp_formula <- JSON_get_Object STR_RESOLUTE_FORMULA resp ;;
@@ -191,7 +169,7 @@ Definition ResoluteResponse_from_JSON `{Jsonifiable Term, Jsonifiable Resolute}
   resultC (mkResoluteResp temp_success formula term).
 
 
-Global Instance Jsonifiable_ResoluteResponse `{Jsonifiable Term, Jsonifiable Resolute}: Jsonifiable ResoluteResponse.
+Global Instance Jsonifiable_ResoluteResponse `{Jsonifiable Term, Jsonifiable Resolute_Formula}: Jsonifiable ResoluteResponse.
 eapply Build_Jsonifiable with
 (to_JSON := ResoluteResponse_to_JSON)
 (from_JSON := ResoluteResponse_from_JSON); unfold ResoluteResponse_to_JSON; unfold ResoluteResponse_from_JSON; solve_json.
