src/Resolute_Types.v
@@ -5,6 +5,6 @@ Require Import Term_Defs Resolute_Logic. (* Attestation_Session AppraisalSummary
 Record ResoluteResponse := 
     mkResoluteResp {
       resoluteresp_success: bool;
-      resoluteresp_formula: Resolute;
+      resoluteresp_formula: Resolute_Formula;
       resoluteresp_term: Term;
   }.
